code/ecdsa/Hacl.Impl.MM.Exponent.fst
@@ -26,10 +26,9 @@ open Spec.ECC
 open Spec.ECC.Curves
 open Hacl.Spec.MontgomeryMultiplication
 
+friend Hacl.Spec.MontgomeryMultiplication
 
 #set-options "--z3rlimit 100"
-
-(* For p256 curve there is a special implementation of multiplication by prime - 2 *)
 
 [@ CInline]
 val cswap: #c: curve -> #m: mode -> bit:uint64{v bit <= 1} -> p: felem c -> q: felem c -> 
@@ -37,13 +36,9 @@ val cswap: #c: curve -> #m: mode -> bit:uint64{v bit <= 1} -> p: felem c -> q: f
   (requires fun h -> as_nat c h p < getModePrime m c /\ as_nat c h q < getModePrime m c /\ 
     live h p /\ live h q /\ eq_or_disjoint p q)
   (ensures  fun h0 _ h1 -> modifies (loc p |+| loc q) h0 h1 /\ (
-    let (r0, r1) = conditional_swap_pow #c bit (as_nat c h0 p) (as_nat c h0 q) in 
-    let pBefore = as_seq h0 p in let qBefore = as_seq h0 q in 
-    let pAfter = as_seq h1 p in let qAfter = as_seq h1 q in 
     as_nat c h1 p < getModePrime m c /\ as_nat c h1 q < getModePrime m c /\
     (v bit == 1 ==> as_seq h1 p == as_seq h0 q /\ as_seq h1 q == as_seq h0 p) /\
     (v bit == 0 ==> as_seq h1 p == as_seq h0 p /\ as_seq h1 q == as_seq h0 q)))
-
 
 let cswap #c #m bit p1 p2 =
   let h0 = ST.get () in
@@ -72,7 +67,6 @@ let cswap #c #m bit p1 p2 =
   Lib.Sequence.eq_intro (as_seq h1 p1) (if v bit = 1 then as_seq h0 p2 else as_seq h0 p1);
   Lib.Sequence.eq_intro (as_seq h1 p2) (if v bit = 1 then as_seq h0 p1 else as_seq h0 p2)
 
-
 inline_for_extraction noextract
 val montgomery_ladder_power_step0: #c: curve -> #m: mode -> a: felem c -> b: felem c -> Stack unit
   (requires fun h -> live h a /\ live h b /\ as_nat c h a < getModePrime m c /\ as_nat c h b < getModePrime m c /\ disjoint a b)
@@ -84,12 +78,15 @@ val montgomery_ladder_power_step0: #c: curve -> #m: mode -> a: felem c -> b: fel
 let montgomery_ladder_power_step0 #c #m a b = 
   let h0 = ST.get() in 
   montgomery_multiplication_buffer #c m a b b;
-  montgomery_square_buffer #c m a a;
+  montgomery_square_buffer #c m a a; 
   let h1 = ST.get() in 
     let aD = fromDomain_ #c #m (as_nat c h0 a) in 
     let bD = fromDomain_ #c #m (as_nat c h0 b) in 
     lemmaToDomainFromDomain #c #m (aD * bD % getModePrime m c);
     lemmaToDomainFromDomain #c #m (aD * aD % getModePrime m c)
+
+
+#set-options "--z3rlimit 300"
 
 
 val montgomery_ladder_power_step: #c: curve -> #m: mode -> a: felem c -> b: felem c 
@@ -102,29 +99,24 @@ val montgomery_ladder_power_step: #c: curve -> #m: mode -> a: felem c -> b: fele
     let a_ = fromDomain_ #c #m (as_nat c h0 a) in 
     let b_ = fromDomain_ #c #m (as_nat c h0 b) in 
     let (r0D, r1D) = _pow_step #c #m (as_seq h0 scalar) (uint_v i) (a_, b_) in 
-    r0D == fromDomain_ #c #m (as_nat c h1 a) /\ r1D == fromDomain_ #c #m (as_nat c h1 b) /\ 
-    as_nat c h1 a < getModePrime m c /\ as_nat c h1 b < getModePrime m c))  
+    r0D == fromDomain_ #c #m (as_nat c h1 a) /\ r1D == fromDomain_ #c #m (as_nat c h1 b) /\
+    as_nat c h1 a < getModePrime m c /\ as_nat c h1 b < getModePrime m c ))  
 
-let montgomery_ladder_power_step #c #m a b scalar i = 
+let montgomery_ladder_power_step #c #m p q scalar i = 
     let h0 = ST.get() in 
-  let bit0 = getScalarLen c -. 1ul -. i in  
+  let bit0 = getScalarLen c -! 1ul -! i in  
   let bit = scalar_bit #c scalar bit0 in 
-  cswap #c #m bit a b;
-  montgomery_ladder_power_step0 #c #m a b;
-  cswap #c #m bit a b;
-  lemma_swaped_steps #c #m (fromDomain_ #c #m (as_nat c h0 a)) (fromDomain_ #c #m (as_nat c h0 b))
-  
+  cswap #c #m bit p q;
+    let h1 = ST.get() in 
+  montgomery_ladder_power_step0 #c #m p q;
+    let h2 = ST.get() in 
+  cswap #c #m bit p q;
+    let h3 = ST.get() in 
 
-val _montgomery_ladder_power: #c: curve -> #m: mode -> a: felem c -> b: felem c 
-  -> scalar: glbuffer uint8 (getScalarLenBytes c) -> Stack unit
-  (requires fun h -> live h a /\ live h b /\ live h scalar /\ as_nat c h a < getModePrime m c /\ 
-    as_nat c h b < getModePrime m c /\ disjoint a b /\ disjoint a scalar /\ disjoint b scalar)
-  (ensures fun h0 _ h1 -> modifies (loc a |+| loc b) h0 h1 /\ (
-    let a_ = fromDomain_ #c #m (as_nat c h0 a) in 
-    let b_ = fromDomain_ #c #m (as_nat c h0 b) in 
-    let (r0D, r1D) = Lib.LoopCombinators.repeati (v (getScalarLen c)) (_pow_step #c #m (as_seq h0 scalar)) (a_, b_) in 
-    r0D == fromDomain #c (as_nat c h1 a) /\ r1D == fromDomain #c (as_nat c h1 b) /\
-    as_nat c h1 a < getModePrime m c /\ as_nat c h1 b < getModePrime m c))
+  let p0D, q0D = (fromDomain_ #c #m (as_nat c h0 p)), (fromDomain_ #c #m (as_nat c h0 q)) in 
+  lemma_swaped_steps #c #m p0D q0D
+
+
 
 let _montgomery_ladder_power #c #m a b scalar = 
   let scalarLen = getScalarLen c in 
@@ -132,54 +124,49 @@ let _montgomery_ladder_power #c #m a b scalar =
     [@inline_let]
     let spec_exp h0 = _pow_step #c #m (as_seq h0 scalar) in 
     [@inline_let]
-    let acc (h: mem) : GTot (tuple2 (elem (getModePrime m c)) (elem (getModePrime m c))) = fromDomain_ #c #m (as_nat c h a), fromDomain_ #c #m (as_nat c h b) in
+    let acc (h: mem) : GTot (tuple2 (elem (getModePrime m c)) (elem (getModePrime m c))) = 
+      fromDomain_ #c #m (as_nat c h a), fromDomain_ #c #m (as_nat c h b) in
 
+    [@inline_let]
+    let inv h (i: nat {i <= v (getScalarLen c)}) = live h a /\ live h b /\ live h scalar /\ modifies (loc a |+| loc b) h0 h /\ 
+      as_nat c h a < getModePrime m c /\ as_nat c h b < getModePrime m c /\
+      acc h == Lib.LoopCombinators.repeati i (spec_exp h0) (acc h0) in 
+ 
   Lib.LoopCombinators.eq_repeati0 (v (getScalarLen c)) (spec_exp h0) (acc h0);
-  [@inline_let]
-  let inv h (i: nat {i <= v (getScalarLen c)}) = live h a /\ live h b /\ live h scalar /\ modifies (loc a |+| loc b) h0 h /\ 
-    as_nat c h a < getModePrime m c /\ as_nat c h b < getModePrime m c /\
-    acc h == Lib.LoopCombinators.repeati i (spec_exp h0) (acc h0) in 
-  admit();
   for 0ul scalarLen inv (fun i -> 
     montgomery_ladder_power_step #c #m a b scalar i;
-    Lib.LoopCombinators.unfold_repeati (v (getScalarLen c)) (spec_exp h0) (acc h0) (uint_v i)
-    );
-    
-  admit()
+    Lib.LoopCombinators.unfold_repeati (v (getScalarLen c)) (spec_exp h0) (acc h0) (uint_v i))
 
 
-val montgomery_ladder_power: #c: curve -> #m: mode -> a: felem c 
-  -> scalar: glbuffer uint8 (getScalarLenBytes c) -> result: felem c -> 
-  Stack unit 
-  (requires fun h -> live h a /\ live h scalar /\ live h result /\ as_nat c h a < getPrime c /\ disjoint a scalar)
-  (ensures fun h0 _ h1 -> modifies (loc a |+| loc result) h0 h1 /\ as_nat c h1 result < getPrime c /\ (
-    let r0D = pow_spec #c #m (as_seq h0 scalar) (fromDomain #c (as_nat c h0 a)) in 
-    let k = fromDomain #c (as_nat c h0 a) in 
-    let scalar = as_seq h0 scalar in 
-    let prime = getPrime c in 
-    as_nat c h1 result = toDomain #c ((pow k (Lib.ByteSequence.nat_from_bytes_le scalar)) % getPrime c) /\
-    r0D == fromDomain #c (as_nat c h1 result)))
+inline_for_extraction noextract 
+val upload_one_montg_form: #c: curve -> #m: mode -> b: felem c -> Stack unit
+  (requires fun h -> live h b)
+  (ensures fun h0 _ h1 -> modifies (loc b) h0 h1 /\ as_nat c h1 b == toDomain_ #c #m 1)
+
+let upload_one_montg_form #c #m b = 
+  match m with 
+  |DH -> Hacl.Impl.EC.LowLevel.upload_one_montg_form b
+  |DSA -> Hacl.Impl.ECDSA.LowLevel.upload_one_montg_form b
+
 
 let montgomery_ladder_power #c #m a scalar result = 
   push_frame(); 
   let len = getCoordinateLenU64 c in 
   let p = create len (u64 0) in  
     lemma_create_zero_buffer (v (getCoordinateLenU64 c)) c;
-  upload_one_montg_form #c p; 
+  upload_one_montg_form #c #m p; 
     lemmaToDomain #c #m 1;
     let h0 = ST.get() in 
   _montgomery_ladder_power #c #m p a scalar;
-    lemmaToDomainFromDomain #c #m 1;  
+    let h1 = ST.get() in 
   copy result p;
-  let h1 = ST.get() in admit();
-  assert(
-    let k = as_seq h0 scalar in 
-    let a = fromDomain #c (as_nat c h0 a) in 
-    let r0D = pow_spec #c #m k a in 
-    
-    r0D == pow a (Lib.ByteSequence.nat_from_bytes_le k) % getPrime c /\
-    r0D == fromDomain #c (as_nat c h1 result));
+  
+  assert( 
+    let b_ = fromDomain_ #c #m (as_nat c h0 a) in 
+    let r0D = pow_spec #c #m (as_seq h0 scalar) (fromDomain_ #c #m (as_nat c h0 a)) in 
+    r0D == fromDomain_ #c #m (as_nat c h1 p));
 
-  lemmaFromDomainToDomain #c #m (as_nat c h1 result); 
+  lemmaFromDomainToDomain #c #m (as_nat c h1 p); 
+
   pop_frame()  
 
