code/ecdsa/Hacl.Impl.MM.Exponent.fsti
@@ -1,0 +1,56 @@
+module Hacl.Impl.MM.Exponent
+
+open FStar.HyperStack.All
+open FStar.HyperStack
+module ST = FStar.HyperStack.ST
+
+open Lib.Sequence
+open Lib.IntTypes
+open Lib.Buffer
+
+open FStar.Math.Lemmas
+
+open Hacl.Impl.EC.LowLevel 
+
+open FStar.Mul
+
+open Lib.Loops
+
+open Hacl.Impl.EC.MontgomeryMultiplication
+open Hacl.Spec.MontgomeryMultiplication
+
+open Hacl.Spec.EC.Definition
+open Hacl.Lemmas.P256
+open Spec.ECDSA.Lemmas
+open Spec.ECC
+open Spec.ECC.Curves
+open Hacl.Spec.MontgomeryMultiplication
+
+#set-options "--z3rlimit 100"
+
+
+val _montgomery_ladder_power: #c: curve -> #m: mode -> a: felem c -> b: felem c 
+  -> scalar: glbuffer uint8 (getScalarLenBytes c) -> Stack unit
+  (requires fun h -> live h a /\ live h b /\ live h scalar /\ as_nat c h a < getModePrime m c /\ 
+    as_nat c h b < getModePrime m c /\ disjoint a b /\ disjoint a scalar /\ disjoint b scalar)
+  (ensures fun h0 _ h1 -> modifies (loc a |+| loc b) h0 h1 /\ (
+    let a_ = fromDomain_ #c #m (as_nat c h0 a) in 
+    let b_ = fromDomain_ #c #m (as_nat c h0 b) in 
+    let (r0D, r1D) = Lib.LoopCombinators.repeati (v (getScalarLen c)) (_pow_step #c #m (as_seq h0 scalar)) (a_, b_) in 
+    r0D == fromDomain_ #c #m (as_nat c h1 a) /\ r1D == fromDomain_ #c #m (as_nat c h1 b) /\
+    as_nat c h1 a < getModePrime m c /\ as_nat c h1 b < getModePrime m c))
+
+  
+val montgomery_ladder_power: #c: curve -> #m: mode -> a: felem c 
+  -> scalar: glbuffer uint8 (getScalarLenBytes c) -> result: felem c -> 
+  Stack unit 
+  (requires fun h -> live h a /\ live h scalar /\ live h result /\ as_nat c h a < getModePrime m c /\
+    disjoint a scalar)
+  (ensures fun h0 _ h1 -> modifies (loc a |+| loc result) h0 h1 /\ 
+    as_nat c h1 result < getModePrime m c /\ (
+    let r0D = pow_spec #c #m (as_seq h0 scalar) (fromDomain_ #c #m (as_nat c h0 a)) in 
+    let k = fromDomain_ #c #m (as_nat c h0 a) in 
+    let scalar = as_seq h0 scalar in 
+    let prime = getModePrime m c in 
+    as_nat c h1 result = toDomain_ #c #m ((pow k (Lib.ByteSequence.nat_from_bytes_le scalar)) % prime) /\ 
+    r0D == fromDomain_ #c #m (as_nat c h1 result)))
